core/PoorTraceLink.v
@@ -1,0 +1,99 @@
+Require Import String.
+
+Require Import core.utils.Utils.
+Require Import core.Model.
+Require Import core.TransformationConfiguration.
+
+(** * Syntax
+
+      In this section, we introduce _one possible_ abstract syntax of the CoqTL transformation engine.  
+      ---- *)
+
+Section TraceLink.
+
+Context {tc: TransformationConfiguration}.
+
+(** ** Traces 
+
+        We introduce the concept of trace in the syntax to track relationship of a produced element (target) and 
+        the source pattern that generates it.   *)
+
+Record TraceLink : Type :=
+  buildTraceLink  
+    { 
+      source : InputPiece * nat * string ;
+      produced : TargetElementType 
+    }.
+
+Definition getSourcePattern (tl: TraceLink):=
+  match tl.(source) with 
+    (sp, i, n)  => sp
+  end.
+
+Definition getIteration (tl: TraceLink):=
+  match tl.(source) with 
+    (sp, i, n)  => i
+  end.
+
+Definition getName (tl: TraceLink):=
+  match tl.(source) with 
+     (sp, i, n) => n
+  end.
+
+Open Scope bool_scope.
+
+
+Definition source_compare (s:InputPiece * nat * string) (t:TraceLink) : bool :=
+  match s with 
+    (e,i,n) =>
+      list_beq tc.(SourceElement_eqb) (getSourcePattern t) e
+      && Nat.eqb (getIteration t) i
+      && String.eqb (getName t) n
+  end.
+
+
+
+Lemma source_compare_refl : 
+  (forall a,  SourceElement_eqb a a = true) ->
+  forall a b, 
+    source_compare a {| source := a ; produced := b |} = true.
+Proof.
+  intros R a b.
+  destruct a as ((l & i) & n). 
+  simpl.
+  unfold getSourcePattern, getIteration, getName ; simpl.
+  rewrite list_beq_refl ; [ | exact R].
+  rewrite NPeano.Nat.eqb_refl.
+  rewrite String.eqb_refl. 
+  reflexivity.
+Qed.
+
+(* Not Used *)
+(* The requirement is too strong for the general case *)
+Lemma source_compare_correct :
+  (forall a b : Metamodel.ElementType SourceMetamodel,
+  Metamodel.elements_eqdec SourceMetamodel a b = true -> a = b) ->
+  forall a b,
+    source_compare a b = true -> b.(source) = a.
+Proof.
+  intro H1.
+  unfold source_compare.
+  intros a b H2 ; destruct a ; destruct p ; destruct b.
+  simpl. destruct source0 ; simpl in *.
+  BoolUtils.destruct_conjunctions.
+  destruct p ; simpl in *.
+  apply EqNat.beq_nat_true in H2 ; subst .
+  apply String.eqb_eq in H0 ; subst.
+  apply list_beq_correct in H ; subst.
+  + reflexivity.
+  + exact H1. 
+Qed.
+
+
+End TraceLink.
+
+Arguments TraceLink {_}.
+
+Arguments source_compare : simpl never.
+
+Notation Trace := (list TraceLink).
